LeanSAT/Reflect/BVExpr/BitBlast/Lemmas/Neg.lean
@@ -1,0 +1,36 @@
+import LeanSAT.Reflect.BVExpr.BitBlast.Lemmas.Basic
+import LeanSAT.Reflect.BVExpr.BitBlast.Lemmas.Add
+import LeanSAT.Reflect.BVExpr.BitBlast.Lemmas.Const
+import LeanSAT.Reflect.BVExpr.BitBlast.Lemmas.Not
+import LeanSAT.Reflect.BVExpr.BitBlast.Impl.Neg
+
+open AIG
+
+namespace BVExpr
+namespace bitblast
+
+open BitVec
+
+theorem blastNeg_eq_eval_getLsb (aig : AIG BVBit) (sub : BVExpr w) (assign : Assignment)
+      (input : RefStream aig w)
+      (hsub : ∀ (idx : Nat) (hidx : idx < w), ⟦aig, input.getRef idx hidx, assign.toAIGAssignment⟧ = (sub.eval assign).getLsb idx)
+    : ∀ (idx : Nat) (hidx : idx < w),
+        ⟦(blastNeg aig input).aig, (blastNeg aig input).stream.getRef idx hidx, assign.toAIGAssignment⟧
+          =
+        (~~~(sub.eval assign) + 1#w).getLsb idx := by
+  intro idx hidx
+  unfold blastNeg
+  dsimp
+  rw [blastAdd_eq_eval_getLsb (lhs := (.un .not sub)) (rhs := (.const 1#w))]
+  . simp
+  . intro idx hidx
+    simp only [RefStream.getRef_cast, Ref_cast', eval_un, BVUnOp.eval_not, getLsb_not, hidx,
+      decide_True, Bool.true_and]
+    rw [AIG.LawfulStreamOperator.denote_mem_prefix (f := blastConst)]
+    rw [blastNot_eq_eval_getLsb]
+    rw [hsub]
+  . intro idx hidx
+    simp
+
+end bitblast
+end BVExpr
